doc-src/TutorialI/Misc/Tree.thy
@@ -8,14 +8,14 @@ Define the datatype of binary trees
 
 datatype 'a tree = Tip | Node "'a tree" 'a "'a tree";(*<*)
 
-consts mirror :: "'a tree \\<Rightarrow> 'a tree";
+consts mirror :: "'a tree \<Rightarrow> 'a tree";
 primrec
 "mirror Tip = Tip"
 "mirror (Node l x r) = Node (mirror r) x (mirror l)";(*>*)
 
 text{*\noindent
 and a function @{term"mirror"} that mirrors a binary tree
-by swapping subtrees (recursively). Prove
+by swapping subtrees recursively. Prove
 *}
 
 lemma mirror_mirror: "mirror(mirror t) = t";
